Updates.

HandbookOfPracticalLogicLean/Chapter2/NF/CNF/ToCNF.lean
@@ -1,7 +1,10 @@
 import MathlibExtraLean.AllPairs
 
 import HandbookOfPracticalLogicLean.Chapter2.NF.NF
-import HandbookOfPracticalLogicLean.Chapter2.NF.DNF.ToDNF_1
+import HandbookOfPracticalLogicLean.Chapter2.NF.Negate
+import HandbookOfPracticalLogicLean.Chapter2.NF.NNF.NNF_1
+import HandbookOfPracticalLogicLean.Chapter2.NF.DNF.ToDNF_3
+
 import HandbookOfPracticalLogicLean.Chapter2.NF.ListConj.Semantics
 import HandbookOfPracticalLogicLean.Chapter2.NF.ListDisj.Semantics
 
@@ -13,15 +16,26 @@ open Formula_
 
 
 /--
-  Helper function for `to_cnf`.
+  Helper function for `to_cnf_v3`.
 -/
-def to_cnf_aux :
+def to_cnf_v3_aux
+  (F : Formula_) :
+  List (List Formula_) :=
+  List.map (fun (l : List Formula_) => List.map negate_literal l) (to_dnf_v3_aux (to_nnf_v1 (not_ F)))
+
+#eval (to_cnf_v3_aux (Formula_| ((p \/ (q /\ r)) /\ (~ p \/ ~ r)))).toString
+
+
+/--
+  Helper function for `to_cnf_v3`.
+-/
+def to_cnf_v3_aux_alt :
   Formula_ → List (List Formula_)
-  | and_ p q => (to_cnf_aux p) ∪ (to_cnf_aux q)
-  | or_ p q => all_pairs_v4 List.union (to_cnf_aux p) (to_cnf_aux q)
+  | and_ p q => (to_cnf_v3_aux_alt p) ∪ (to_cnf_v3_aux_alt q)
+  | or_ p q => all_pairs_v4 List.union (to_cnf_v3_aux_alt p) (to_cnf_v3_aux_alt q)
   | F => [[F]]
 
-#eval (to_cnf_aux (Formula_| ((p \/ (q /\ r)) /\ (~ p \/ ~ r)))).toString
+#eval (to_cnf_v3_aux_alt (Formula_| ((p \/ (q /\ r)) /\ (~ p \/ ~ r)))).toString
 
 
 /--
@@ -34,111 +48,110 @@ def list_of_lists_to_conjunction_of_disjunctions
 
 
 /--
-  `to_cnf F` := Translates the formula `F` to a logically equivalent formula. If `F` is in negation normal form then `to_cnf F` is in conjunctive normal form.
+  `to_cnf_v3 F` := Translates the formula `F` to a logically equivalent formula. If `F` is in negation normal form then `to_cnf_v3 F` is in conjunctive normal form.
 -/
-def to_cnf
+def to_cnf_v3
   (F : Formula_) :
   Formula_ :=
-  list_of_lists_to_conjunction_of_disjunctions (to_cnf_aux F)
+  list_of_lists_to_conjunction_of_disjunctions (to_cnf_v3_aux F)
 
 
 #eval (list_of_lists_to_conjunction_of_disjunctions [[atom_ "P", atom_ "Q"], [not_ (atom_ "P"), atom_ "R"]]).toString
 
 
-lemma eval_eq_eval_to_cnf
+lemma eval_eq_eval_to_cnf_v3
   (V : ValuationAsTotalFunction)
   (F : Formula_) :
-  eval V F = true ↔ eval V (to_cnf F) = true :=
+  eval V F = true ↔ eval V (to_cnf_v3 F) = true :=
   by
-  unfold to_cnf
+  unfold to_cnf_v3
   induction F
   case and_ phi psi phi_ih psi_ih =>
     unfold list_of_lists_to_conjunction_of_disjunctions at phi_ih
 
     unfold list_of_lists_to_conjunction_of_disjunctions at psi_ih
 
-    unfold to_cnf_aux
+    unfold to_cnf_v3_aux
     unfold list_of_lists_to_conjunction_of_disjunctions
     simp only [eval]
     simp only [bool_iff_prop_and]
     rewrite [phi_ih]
     rewrite [psi_ih]
     simp only [eval_list_conj_eq_true_iff_forall_eval_eq_true]
-    simp only [List.mem_map, List.mem_union_iff]
+    simp only [List.mem_map]
     constructor
-    · intro a1
+    · intro a1 F a2
       obtain ⟨a1_left, a1_right⟩ := a1
-      intro F a2
-      obtain ⟨FS, a2_left, a2_right⟩ := a2
-      cases a2_left
-      case inl a2_left =>
+
+      obtain ⟨FS, ⟨PS, a2_left_left, a2_left_right⟩, a2_right⟩ := a2
+      simp only [to_nnf_v1] at a2_left_left
+      simp only [to_nnf_neg_v1] at a2_left_left
+      unfold to_dnf_v3_aux at a2_left_left
+      simp only [List.mem_union_iff] at a2_left_left
+
+      cases a2_left_left
+      case inl a2_left_left =>
         apply a1_left
         apply Exists.intro FS
-        exact ⟨a2_left, a2_right⟩
-      case inr a2_left =>
+        constructor
+        · unfold to_cnf_v3_aux
+          simp only [List.mem_map]
+          unfold to_nnf_v1
+          apply Exists.intro PS
+          exact ⟨a2_left_left, a2_left_right⟩
+        · exact a2_right
+      case inr a2_left_left =>
         apply a1_right
         apply Exists.intro FS
-        exact ⟨a2_left, a2_right⟩
+        constructor
+        · unfold to_cnf_v3_aux
+          simp only [List.mem_map]
+          unfold to_nnf_v1
+          apply Exists.intro PS
+          exact ⟨a2_left_left, a2_left_right⟩
+        · exact a2_right
     · intro a1
       constructor
       · intro F a2
         obtain ⟨FS, a2_left, a2_right⟩ := a2
+        unfold to_cnf_v3_aux at a2_left
+        simp only [List.mem_map] at a2_left
+        obtain ⟨PS, a2_left_left, a2_left_right⟩ := a2_left
+        unfold to_nnf_v1 at a2_left_left
+
         apply a1
         apply Exists.intro FS
         constructor
-        · left
-          exact a2_left
+        · unfold to_nnf_v1
+          unfold to_nnf_neg_v1
+          unfold to_dnf_v3_aux
+          simp only [List.mem_union_iff]
+          apply Exists.intro PS
+          constructor
+          · left
+            exact a2_left_left
+          · exact a2_left_right
         · exact a2_right
       · intro F a2
         obtain ⟨FS, a2_left, a2_right⟩ := a2
+        unfold to_cnf_v3_aux at a2_left
+        simp only [List.mem_map] at a2_left
+        obtain ⟨PS, a2_left_left, a2_left_right⟩ := a2_left
+        unfold to_nnf_v1 at a2_left_left
+
         apply a1
         apply Exists.intro FS
         constructor
-        · right
-          exact a2_left
+        · unfold to_nnf_v1
+          unfold to_nnf_neg_v1
+          unfold to_dnf_v3_aux
+          simp only [List.mem_union_iff]
+          apply Exists.intro PS
+          constructor
+          · right
+            exact a2_left_left
+          · exact a2_left_right
         · exact a2_right
-  case or_ phi psi phi_ih psi_ih =>
-    unfold list_of_lists_to_conjunction_of_disjunctions at phi_ih
-
-    unfold list_of_lists_to_conjunction_of_disjunctions at psi_ih
-
-    unfold to_cnf_aux
-    unfold list_of_lists_to_conjunction_of_disjunctions
-    simp only [eval]
-    simp only [bool_iff_prop_or]
-    rewrite [phi_ih]
-    rewrite [psi_ih]
-    simp only [eval_list_conj_eq_true_iff_forall_eval_eq_true]
-    simp only [List.mem_map]
-    simp only [mem_all_pairs_v4_union_iff_eq_union]
-    constructor
-    · intro a1 F a2
-      obtain ⟨FS, ⟨PS, QS, ⟨PS_mem, QS_mem, a2_left⟩⟩, a2_right⟩ := a2
-      rewrite [← a2_right]
-      rewrite [← a2_left]
-      simp only [eval_list_disj_union]
-      cases a1
-      case inl a1 =>
-        left
-        apply a1
-        apply Exists.intro PS
-        constructor
-        · exact PS_mem
-        · rfl
-      case inr a1 =>
-        right
-        apply a1
-        apply Exists.intro QS
-        constructor
-        · exact QS_mem
-        · rfl
-    · intro a1
-      simp? at a1
-      simp?
-      clear phi_ih
-      clear psi_ih
-      simp only [eval_list_disj_eq_true_iff_exists_eval_eq_true]
-      sorry
   all_goals
     sorry
 
